\documentclass[]{article}

\usepackage{amsfonts}

%opening
\title{Continuous Finance HW1}
\author{Lisa He}

\begin{document}

\maketitle {}


\section{Problem 4}
$\Delta B_{i} \sim N(0, t_{i+1}-t{i})$ 

So,  $(\Delta B_{i}^{2}) = var(\Delta B_{i}) = \Delta t_{i}$

$\mathbb{E} (\Delta B_{i}^{4}) = 3var(\Delta B_{i})^{2} = 3(\Delta t_{i} )^{2}$

Therefore, \\ $LHS = 
\mathbb{E} [(\Delta B_{i})^{4}-2(\Delta B_{i})^{2}\Delta t_{i}+(\Delta t_{i})^{2}\parallel F_{t_{i}}] \\
= 3(\Delta t_{i} )^{2}-2(\Delta t_{i} )^{2}+ (\Delta t_{i} )^{2} \\
= 2(\Delta t_{i} )^{2}\\
= RHS$
\\

$\[ p_t(x, y) = f_t(y - x) =\frac{1}{\sigma \sqrt{2 \pi t}} \exp\left[-\frac{1}{2 \sigma^2 t} (y - x - \mu t)^2\right], \quad t \in (0, \infty); \; x, \, y \in \R \]$
\end{document}
